New model for refcell, in order to prove map_split.

theories/typing/lib/refcell/refcell.v
@@ -6,24 +6,35 @@ From lrust.typing Require Import typing.
 Set Default Proof Using "Type".
 
 Definition refcell_stR :=
-  optionUR (prodR (agreeR lftC) (csumR (exclR unitC) (prodR fracR positiveR))).
+  optionUR (prodR (prodR
+             (agreeR (prodC lftC boolC))
+             fracR)
+             positiveR).
 Class refcellG Σ :=
   RefCellG :> inG Σ (authR refcell_stR).
 Definition refcellΣ : gFunctors := #[GFunctor (authR refcell_stR)].
 Instance subG_refcellΣ {Σ} : subG refcellΣ Σ → refcellG Σ.
 Proof. solve_inG. Qed.
 
-Definition Z_of_refcell_st (st : refcell_stR) : Z :=
+Definition refcell_st := option ((lft * Datatypes.bool) * frac * positive).
+Definition refcell_st_to_R (st : refcell_st) : refcell_stR :=
+  match st with
+  | None => None
+  | Some (x, q, n) => Some (to_agree x, q, n)
+  end.
+Coercion refcell_st_to_R : refcell_st >-> ucmra_car.
+
+Definition Z_of_refcell_st (st : refcell_st) : Z :=
   match st with
   | None => 0
-  | Some (_, Cinr (_, n)) => Zpos n
-  | Some _ => -1
+  | Some (_, false, _, n) => Zpos n (* Immutably borrowed *)
+  | Some (_, true, _, n) => Zneg n  (* Mutably borrowed *)
   end.
 
-Definition reading_st (q : frac) (ν : lft) : refcell_stR :=
-  Some (to_agree ν, Cinr (q, xH)).
-Definition writing_st (ν : lft) : refcell_stR :=
-  Some (to_agree ν, Cinl (Excl ())).
+Definition reading_stR (q : frac) (ν : lft) : refcell_stR :=
+  refcell_st_to_R $ Some (ν, false, q, xH).
+Definition writing_stR (q : frac) (ν : lft) : refcell_stR :=
+  refcell_st_to_R $ Some (ν, true, q, xH).
 
 Definition refcellN := lrustN .@ "refcell".
 Definition refcell_invN := refcellN .@ "inv".
@@ -32,21 +43,16 @@ Section refcell_inv.
   Context `{typeG Σ, refcellG Σ}.
 
   Definition refcell_inv tid (l : loc) (γ : gname) (α : lft) ty : iProp Σ :=
-    (∃ st, l ↦ #(Z_of_refcell_st st) ∗ own γ (● st) ∗
+    (∃ st, l ↦ #(Z_of_refcell_st st) ∗ own γ (● (refcell_st_to_R st)) ∗
       match st return _ with
       | None =>
         (* Not borrowed. *)
         &{α}((l +ₗ 1) ↦∗: ty.(ty_own) tid)
-      | Some (agν, st) =>
-        ∃ ν, agν ≡ to_agree ν ∗
-             (1.[ν] ={↑lftN,∅}▷=∗ &{α}((l +ₗ 1) ↦∗: ty.(ty_own) tid)) ∗
-             match st with
-             | Cinr (q, n) =>
-               (* Immutably borrowed. *)
-               ty.(ty_shr) (α ⊓ ν) tid (l +ₗ 1) ∗
-               ∃ q', ⌜(q + q')%Qp = 1%Qp⌝ ∗ q'.[ν]
-             | _ => (* Mutably borrowed. *) True
-             end
+      | Some (ν, rw, q, _) =>
+        (1.[ν] ={↑lftN,∅}▷=∗ &{α}((l +ₗ 1) ↦∗: ty.(ty_own) tid)) ∗
+        (∃ q', ⌜(q + q')%Qp = 1%Qp⌝ ∗ q'.[ν]) ∗
+        if rw then (* Mutably borrowed. *) True
+        else       (* Immutably borrowed. *) ty.(ty_shr) (α ⊓ ν) tid (l +ₗ 1)
       end)%I.
 
   Global Instance refcell_inv_type_ne n tid l γ α :
@@ -68,7 +74,7 @@ Section refcell_inv.
     refcell_inv tid l γ α ty1 -∗ refcell_inv tid l γ α ty2).
   Proof.
     (* TODO : this proof is essentially [solve_proper], but within the logic. *)
-  (*             It would easily gain from some automation. *)
+    (*             It would easily gain from some automation. *)
     rewrite eqtype_unfold. iIntros (Hty) "HL".
     iDestruct (Hty with "HL") as "#Hty". iIntros "* !# #HE H".
     iDestruct ("Hty" with "HE") as "(% & #Hown & #Hshr)".
@@ -78,12 +84,12 @@ Section refcell_inv.
       iNext; iAlways; iSplit; iIntros "H"; iDestruct "H" as (vl) "[Hf H]"; iExists vl;
       iFrame; by iApply "Hown". }
     iDestruct "H" as (st) "H"; iExists st;
-      iDestruct "H" as "($&$&H)"; destruct st as [[agν st]|]; try done;
+      iDestruct "H" as "($&$&H)"; destruct st as [[[[ν rw] q' ] n]|]; try done;
       last by iApply "Hb".
-    iDestruct "H" as (ν) "(Hag & Hh & H)". iExists ν. iFrame. iSplitL "Hh".
+    iDestruct "H" as "(Hh & $ & H)". iSplitL "Hh".
     { iIntros "Hν". iMod ("Hh" with "Hν") as "Hh". iModIntro. iNext.
       iMod "Hh". by iApply "Hb". }
-    destruct st as [|[]|]; try done. iDestruct "H" as "[H $]". by iApply "Hshr".
+    destruct rw; try done. by iApply "Hshr".
   Qed.
 End refcell_inv.
 
@@ -101,40 +107,38 @@ Section refcell.
     {| ty_size := S ty.(ty_size);
        ty_own tid vl :=
          match vl return _ with
-         | #(LitInt z) :: vl' => ⌜-1 ≤ z⌝ ∗ ty.(ty_own) tid vl'
+         | #(LitInt z) :: vl' => ty.(ty_own) tid vl'
          | _ => False
          end%I;
        ty_shr κ tid l :=
          (∃ α γ, κ ⊑ α ∗ &na{α, tid, refcell_invN}(refcell_inv tid l γ α ty))%I |}.
   Next Obligation.
-    iIntros (??[|[[]|]]); try iIntros "[]". rewrite ty_size_eq.
-    iIntros "[_ %] !% /=". congruence.
+    iIntros (??[|[[]|]]); try iIntros "[]". rewrite ty_size_eq /=. by iIntros (->).
   Qed.
   Next Obligation.
     iIntros (ty E κ l tid q ?) "#LFT Hb Htok".
     iMod (bor_acc_cons with "LFT Hb Htok") as "[H Hclose]". done.
     iDestruct "H" as ([|[[| |n]|]vl]) "[H↦ H]"; try iDestruct "H" as ">[]".
-    iDestruct "H" as "[>% Hown]".
-    iMod ("Hclose" $! ((∃ n:Z, l ↦ #n ∗ ⌜-1 ≤ n⌝) ∗
+    iDestruct "H" as "Hown".
+    iMod ("Hclose" $! ((∃ n:Z, l ↦ #n) ∗
             (l +ₗ 1) ↦∗: ty.(ty_own) tid) with "[] [-]")%I as "[H [Htok Htok']]".
-    { iIntros "!> [Hn Hvl] !>". iDestruct "Hn" as (n') "[Hn >%]".
+    { iIntros "!> [Hn Hvl] !>". iDestruct "Hn" as (n') "Hn".
       iDestruct "Hvl" as (vl') "[H↦ Hvl]".
-      iExists (#n'::vl'). rewrite heap_mapsto_vec_cons. iFrame "∗%". }
+      iExists (#n'::vl'). rewrite heap_mapsto_vec_cons. iFrame. }
     { iNext. rewrite heap_mapsto_vec_cons. iDestruct "H↦" as "[Hn Hvl]".
-      iSplitL "Hn"; [eauto|iExists _; iFrame]. }
+      iSplitL "Hn"; eauto with iFrame. }
     iMod (bor_sep with "LFT H") as "[Hn Hvl]". done.
     iMod (bor_acc_cons with "LFT Hn Htok") as "[H Hclose]". done.
     iAssert ((q / 2).[κ] ∗ ▷ ∃ γ, refcell_inv tid l γ κ ty)%I with "[> -Hclose]"
       as "[$ HQ]"; last first.
     { iMod ("Hclose" with "[] HQ") as "[Hb $]".
-      - iIntros "!> H !>". iNext. iDestruct "H" as (γ st) "(H & _ & _)".
-        iExists _. iIntros "{$H}!%". destruct st as [[?[|[]|]]|]; simpl; lia.
+      - iIntros "!> H !>". iNext. iDestruct "H" as (γ st) "(H & _ & _)". eauto.
       - iMod (bor_exists with "LFT Hb") as (γ) "Hb". done.
         iExists κ, γ. iSplitR. by iApply lft_incl_refl. by iApply bor_na. }
-    clear dependent n. iDestruct "H" as ([|n|[]]) "[Hn >%]"; try lia.
+    clear dependent n. iDestruct "H" as ([|n|n]) "Hn"; try lia.
     - iFrame. iMod (own_alloc (● None)) as (γ) "Hst". done. iExists γ, None. by iFrame.
     - iMod (lft_create with "LFT") as (ν) "[[Htok1 Htok2] #Hhν]". done.
-      iMod (own_alloc (● Some (to_agree ν, Cinr ((1/2)%Qp, n)))) as (γ) "Hst".
+      iMod (own_alloc (● (refcell_st_to_R $ Some (ν, false, (1/2)%Qp, n)))) as (γ) "Hst".
       { by apply auth_auth_valid. }
       iApply (fupd_mask_mono (↑lftN)); first done.
       iMod (rebor _ _ (κ ⊓ ν) with "LFT [] Hvl") as "[Hvl Hh]". done.
@@ -142,14 +146,16 @@ Section refcell.
       iDestruct (lft_intersect_acc with "Htok' Htok1") as (q') "[Htok Hclose]".
       iMod (ty_share with "LFT Hvl Htok") as "[Hshr Htok]". done.
       iDestruct ("Hclose" with "Htok") as "[$ Htok]".
-      iExists γ, _. iFrame "Hst Hn". iExists _. iIntros "{$Hshr}".
-      iSplitR; first by auto. iSplitR "Htok2"; last first.
-      { iExists _. iFrame. rewrite Qp_div_2. auto. }
+      iExists γ, _. iFrame "Hst Hn Hshr".
+      iSplitR "Htok2"; last by iExists _; iFrame; rewrite Qp_div_2.
       iIntros "!> !> Hν". iMod ("Hhν" with "Hν") as "Hν". iModIntro. iNext. iMod "Hν".
       iApply fupd_mask_mono; last iApply "Hh". done. rewrite -lft_dead_or. auto.
-    - iMod (own_alloc (● writing_st static)) as (γ) "Hst". { by apply auth_auth_valid. }
-      iFrame. iExists _, _. iFrame. iExists _. iSplitR; first by auto.
-      iIntros "!>!> _". iApply step_fupd_intro; [set_solver|auto].
+    - iMod (own_alloc (● (refcell_st_to_R $ Some (static, true, (1/2)%Qp, n)))) as (γ) "Hst".
+      { by apply auth_auth_valid. }
+      iFrame "Htok'". iExists γ, _. iFrame. iSplitR.
+      { rewrite -step_fupd_intro. auto. set_solver+. }
+      iSplitR; [|done]. iExists (1/2)%Qp. rewrite Qp_div_2. iSplitR; [done|].
+      iApply lft_tok_static.
   Qed.
   Next Obligation.
     iIntros (?????) "#Hκ H". iDestruct "H" as (α γ) "[#??]".
@@ -182,7 +188,7 @@ Section refcell.
     iIntros "!# #HE". iDestruct ("EQ'" with "HE") as "(% & #Hown & #Hshr)".
     iSplit; [|iSplit; iIntros "!# * H"].
     - iPureIntro. simpl. congruence.
-    - destruct vl as [|[[]|]]; try done. iDestruct "H" as "[$ H]". by iApply "Hown".
+    - destruct vl as [|[[]|]]; try done. by iApply "Hown".
     - iDestruct "H" as (a γ) "[Ha H]". iExists a, γ. iFrame.
       iApply na_bor_iff; last done. iNext; iAlways; iSplit; iIntros "H".
       by iApply "Hty1ty2". by iApply "Hty2ty1".
@@ -198,7 +204,7 @@ Section refcell.
 
   Global Instance refcell_send :
     Send ty → Send (refcell ty).
-  Proof. move=>????[|[[]|]]//=??. iIntros "[$?]". by iApply send_change_tid. Qed.
+  Proof. move=>????[|[[]|]]//=. Qed.
 End refcell.
 
 Hint Resolve refcell_mono' refcell_proper' : lrust_typing.
